upd

Computation.v
@@ -1,480 +1,248 @@
-Require Import List Relations Arith Alphabet Bool Language Lia.
+Require Import List Arith Alphabet Language Lia.
+
+Definition transition (state: Type) := state -> state + nat.
 
 Section Computation.
   Context {state: Type}.
-  Variable step_rel: relation state.
-  Variable accepting_state: state -> Prop.
-  Variable encode_input: bitstr -> state.
-
-  Definition deterministic :=
-    forall (s s' s'': state), step_rel s s' -> step_rel s s'' -> s' = s''.
+  Variable next: transition state.
+  Variable encode_input: nat -> state.
 
   Record decision_model :=
-    { dm_step: relation state; dm_acc: state -> Prop; dm_enc: bitstr -> state }.
+    { dm_next: transition state; dm_enc: nat -> state }.
   Definition dm_class := decision_model -> Prop.
 
-  Inductive steps: relation state :=
+  Inductive steps: state -> state -> Prop :=
   | stepsRefl: forall (s: state), steps s s
   | stepsOnce: forall (s s' s'': state),
-      steps s s' -> step_rel s' s'' -> steps s s''.
+      steps s s' -> next s' = inl s'' -> steps s s''.
 
+  Definition halted (s: state) := exists n, next s = inr n.
 
-  Lemma steps_transitive: forall (s s' s'': state),
-    steps s s' -> steps s' s'' -> steps s s''.
+  Inductive eval: state -> nat -> Prop :=
+  | evalHalted: forall (s: state) (n: nat), next s = inr n -> eval s n
+  | evalStep:
+      forall (s s': state) (n: nat), next s = inl s' -> eval s' n -> eval s n.
+
+  Inductive runtime: state -> nat -> Prop :=
+  | runtimeHalted: forall (s: state), halted s -> runtime s 0
+  | runtimeStep: forall (s s': state) (n: nat), next s = inl s' -> runtime s' n -> runtime s (S n).
+
+  Definition halts (s: state) := exists n, eval s n.
+  Definition halts' (s: state) := exists n, runtime s n.
+
+  Lemma halts_iff_halts': forall (s: state), halts s <-> halts' s.
   Proof.
     intros.
-    induction H0; auto.
-    apply stepsOnce with (s' := s'); auto.
+    split; intros.
+    - destruct H.
+      induction H.
+      + unfold halts'. exists 0. constructor. unfold halted. exists n. auto.
+      + unfold halts' in *. destruct IHeval.
+        exists (S x). econstructor; eauto.
+    - destruct H.
+      induction H.
+      + destruct H. exists x. econstructor; eauto.
+      + destruct IHruntime. exists x. eapply evalStep; eauto.
   Qed.
 
-  Lemma first_step: forall (s s': state),
-    steps s s' -> s = s' \/ exists s'', step_rel s s''.
+  Lemma steps_eval:
+    forall (s s': state) (n: nat), steps s s' -> (decision s b <-> decision s' b).
   Proof.
-    clear accepting_state.
     intros.
     induction H.
     - intuition.
-    - destruct IHsteps.
-      + subst.
-        eauto.
-      + eauto.
+    - rewrite IHsteps. clear IHsteps H s.
+      split; intro.
+      + inversion H; subst; rewrite H0 in H1.
+        * discriminate.
+        * inversion H1. auto.
+      + apply decisionStep with (s' := s''); auto.
   Qed.
 
-  Definition halted (s: state) := forall (s': state), ~step_rel s s'.
-
-  Definition runtime_f (initial: state) (f: state -> nat) :=
-    forall (s s': state), steps initial s -> step_rel s s' -> f s > f s'.
-
-  Lemma runtime_f_monotone:
-    forall f (s s': state), steps s s' -> runtime_f s f -> f s >= f s'.
+  Lemma steps_halts:
+    forall (s s': state), steps s s' -> (halts s <-> halts s').
   Proof.
     intros.
-    unfold runtime_f in H0.
-    induction H.
-    - auto.
-    - remember (IHsteps H0).
-      enough (f s' > f s'').
-      + lia.
-      + apply H0; auto.
+    split; intro.
+    - destruct H0.
+      + apply (steps_decision s s' true H) in H0. unfold halts. auto.
+      + apply (steps_decision s s' false H) in H0. unfold halts. auto.
+    - destruct H0.
+      + apply (steps_decision s s' true H) in H0. unfold halts. auto.
+      + apply (steps_decision s s' false H) in H0. unfold halts. auto.
   Qed.
 
-  Lemma runtime_f_monotone':
-    forall f (s s': state), steps s s' -> runtime_f s f -> runtime_f s' f.
+  Lemma decision_unique: forall (s: state), ~(decision s true /\ decision s false).
   Proof.
-    unfold runtime_f.
-    intros.
-    apply H0; auto.
-    apply steps_transitive with (s' := s'); auto.
-  Qed.
-
-  Definition halts (initial: state) :=
-    exists f, runtime_f initial f.
-
-  Lemma halts_steps_monotone:
-    forall (s s': state), steps s s' -> halts s -> halts s'.
-  Proof.
-    intros.
-    unfold halts in *.
-    destruct H0 as [f].
-    exists f.
-    unfold runtime_f in *.
-    induction H.
-    - exact H0.
-    - intros.
-      apply H0; auto.
-      apply steps_transitive with (s' := s'); auto.
-      apply steps_transitive with (s' := s''); auto.
-      apply stepsOnce with (s' := s'); auto.
-      constructor.
-  Qed.
-
-  Definition halts_within (initial: state) (n: nat) :=
-    exists (f: state -> nat), runtime_f initial f /\ f initial = n.
-
-  Axiom halts_within_constructible:
-    forall (initial: state) (n: nat), halts_within initial n ->
-    { f | runtime_f initial f /\ f initial = n }.
-
-  Lemma halts_within_monotone:
-    forall (initial: state) (n m: nat), n < m ->
-    halts_within initial n -> halts_within initial m.
-  Proof.
-    clear accepting_state.
-    intros.
-    destruct H0 as [f].
-    destruct H0.
-    unfold halts_within.
-    apply Nat.le_exists_sub in H.
+    intros. intro.
     destruct H.
-    destruct H.
-    exists (fun s => x + S (f s)).
-    unfold runtime_f.
-    rewrite H1.
-    intuition.
+    assert (halts' s).
+    - apply halts_iff_halts'. unfold halts. auto.
+    - destruct H1.
+      induction H1.
+      + unfold halted in H1.
+        destruct H1.
+        * inversion H0; subst; rewrite H1 in H2; discriminate.
+        * inversion H; subst; rewrite H1 in H2; discriminate.
+      + inversion H; inversion H0; subst.
+        * rewrite H3 in H6. discriminate.
+        * rewrite H3 in H6. discriminate.
+        * rewrite H3 in H7. discriminate.
+        * rewrite H3 in H7. inversion H7. rewrite H1 in H3. inversion H3. subst.
+          apply IHruntime; auto.
   Qed.
 
-  Lemma halts_within_monotone':
-    forall (initial: state) (n m: nat), n <= m ->
-    halts_within initial n -> halts_within initial m.
+  Definition decides (l: language) :=
+    forall (w: bitstr), halts (encode_input w) /\ (decision (encode_input w) true <-> l w).
+
+  Lemma language_unique: forall (l l': language), decides l -> decides l' -> l = l'.
   Proof.
     intros.
-    apply Nat.lt_eq_cases in H.
-    destruct H.
-    - eapply halts_within_monotone; eauto.
-    - subst. auto.
+    apply lang_extensionality.
+    intro. split; intro; unfold decides in *;
+    specialize H with w; specialize H0 with w; destruct H, H0; intuition.
   Qed.
 
-  Lemma halts_within_step_monotone:
-    forall (s s': state) (t : nat),
-    step_rel s s' -> halts_within s (S t) -> halts_within s' t.
-  Proof.
-    intros.
-    unfold halts_within in H0.
-    destruct H0 as [f].
-    destruct H0.
-    apply halts_within_monotone' with (n := f s').
-    - unfold runtime_f in H0.
-      specialize H0 with s s'.
-      remember (H0 (stepsRefl s) H).
-      lia.
-    - unfold halts_within.
-      exists f. intuition.
-      apply (runtime_f_monotone' f s s'); repeat econstructor; auto.
-  Qed.
+  Fixpoint simulate (s: state) (n: nat): option bool :=
+    match n with
+    | 0 => None
+    | S m => match next s with
+             | inl s' => simulate s' m
+             | inr b => Some b
+             end
+    end.
 
-  Lemma halts_within_steps_monotone:
-    forall (s s': state) (t : nat),
-    steps s s' -> halts_within s t -> halts_within s' t.
-  Proof.
-    intros.
-    unfold halts_within in H0.
-    destruct H0 as [f].
-    destruct H0.
-    assert (halts_within s' (f s')).
-    - exists f.
-      unfold runtime_f in *.
-      intuition.
-      apply H0; intuition.
-      apply steps_transitive with (s' := s'); auto.
-    - destruct (Nat.eq_dec t (f s')).
-      + exists f.
-        unfold runtime_f.
-        intuition.
-        apply H0; intuition.
-        apply steps_transitive with (s' := s'); auto.
-      + apply halts_within_monotone with (n := f s'); auto.
-        rewrite <- H1.
-        rewrite <- H1 in n.
-        remember (runtime_f_monotone f s s' H H0).
-        lia.
-  Qed.
-
-  Lemma halts_halts_within:
-    forall (initial: state), halts initial -> exists (n: nat), halts_within initial n.
-  Proof.
-    intros.
-    destruct H as [f].
-    exists (f initial).
-    unfold halts_within.
-    exists f.
-    auto.
-  Qed.
-
-  Definition runtime (initial: state) (t: nat) :=
-    halts_within initial t /\ forall t', t' < t -> ~halts_within initial t'.
-
-  Lemma runtime_unique:
-    forall (initial: state) (t t': nat),
-    runtime initial t -> runtime initial t' -> t = t'.
-  Proof.
-    intros.
-    destruct (t ?= t') eqn: Hc.
-    - apply Nat.compare_eq_iff in Hc. auto.
-    - exfalso.
-      apply Nat.compare_lt_iff in Hc.
-      unfold runtime in H, H0.
-      destruct H, H0.
-      exact (H2 t Hc H).
-    - exfalso.
-      apply Nat.compare_gt_iff in Hc.
-      unfold runtime in H, H0.
-      destruct H, H0.
-      exact (H1 t' Hc H0).
-  Qed.
-
-  Lemma runtime_zero_halted:
-    forall (s: state),
-    halted s <-> runtime s 0.
-  Proof.
-    unfold halted.
-    unfold runtime.
-    unfold halts_within.
-    unfold runtime_f.
-    intuition.
-    - exists (fun x => 0).
-      intuition.
-      exfalso.
-      remember (first_step s s0 H0) as Ht.
-      destruct Ht.
-      + subst.
-        eapply H. eauto.
-      + destruct e.
-        eapply H. eauto.
-    - lia.
-    - destruct H0 as [f].
-      destruct H0.
-      remember (H0 s s' (stepsRefl s) H).
-      lia.
-  Qed.
-
-  Lemma runtime_step_monotone:
-    forall (s s': state) (t t': nat),
-    runtime s t -> runtime s' t' -> step_rel s s' -> t > t'.
-  Proof.
-    intros.
-    unfold runtime in H, H0.
-    destruct H, H0.
-    destruct t.
-    - assert (runtime s 0).
-      + unfold runtime. intuition.
-      + apply runtime_zero_halted in H4.
-        exfalso.
-        unfold halted in H4.
-        apply (H4 s').
-        auto.
-    - remember (halts_within_step_monotone s s' t H1 H).
-      destruct (S t ?= t') eqn: Hc.
-      + apply Nat.compare_eq_iff in Hc.
-        exfalso.
-        assert (t < t') by lia.
-        exact (H3 t H4 h).
-      + apply Nat.compare_lt_iff in Hc.
-        exfalso.
-        assert (t < t') by lia.
-        exact (H3 t H4 h).
-      + apply Nat.compare_gt_iff in Hc.
-        auto.
-  Qed.
-
-  Definition halts' (input: bitstr) := halts (encode_input input).
-
-  Inductive decision: state -> bool -> Prop :=
-  | decisionRejects: forall (s: state),
-      halts s -> (forall (s': state), steps s s' -> halted s' -> ~accepting_state s') ->
-      decision s false
-  | decisionAccepts: forall (s: state),
-      halts s -> (exists (s': state), steps s s' /\ halted s' /\ accepting_state s') ->
-      decision s true.
-
-  Lemma not_accept_reject: forall (s: state), ~(decision s false /\ decision s true).
-  Proof.
-    intro. intro.
-    destruct H.
-    inversion H. inversion H0. subst. clear H H0.
-    destruct H5.
-    specialize H2 with x.
-    intuition.
-  Qed.
-
-  Definition decision' (w: bitstr) (b: bool) := decision (encode_input w) b.
-  Definition rejects (w: bitstr) := decision' w false.
-  Definition accepts (w: bitstr) := decision' w true.
-
-  Lemma not_accept_reject': forall (w: bitstr), ~(rejects w /\ accepts w).
-  Proof.
-    intro.
-    unfold rejects.
-    unfold decision'.
-    apply not_accept_reject.
-  Qed.
-
-  Definition next_steps_exists :=
-    { f: state -> list state | forall (s s': state), step_rel s s' <-> In s' (f s)}.
-
-  Lemma runtime_tight:
-    next_steps_exists ->
-    forall (s: state) (t: nat),
-    runtime s (S t) -> exists (s': state), step_rel s s' /\ runtime s' t.
-  Proof.
-    intros.
-    destruct X as [f Hf].
-    remember (Hf s) as Hfs. clear HeqHfs Hf.
-  Admitted.
-
-  Local Definition inductive_runtime_f (s: state) (t: nat)
-    (H: forall (s': state), {halts_within s' t} + {~halts_within s' t}): state -> nat.
-    intro s'.
-    destruct (H s').
-    - apply halts_within_constructible in h.
-      destruct h as [f].
-      exact (f s').
-    - exact (S t).
-  Defined.
-
-  Local Lemma inductive_runtime_f_correct:
-    forall (s: state) (t: nat)
-    (H: forall (s': state), {halts_within s' t} + {~halts_within s' t})
-    (H': forall s' : state, step_rel s s' -> halts_within s' t),
-    runtime_f s (inductive_runtime_f s t H).
-  Proof.
-    intros.
-    unfold runtime_f.
-    intros.
-    unfold inductive_runtime_f.
-    apply first_step in H0.
-    destruct H0, (H s0), (H s'); repeat destruct halts_within_constructible.
-    - destruct a, a0.
-      unfold runtime_f in H2.
-      specialize H2 with s0 s'.
-      remember (H2 (stepsRefl s0) H1).
-
-  Admitted.
-
-  Local Lemma halts_within_comp:
-    next_steps_exists ->
-    forall (s: state) (t t': nat), t < t' -> {halts_within s t} + {~halts_within s t}.
-  Proof.
-    intros.
-    destruct X as [f Hf].
-    revert s.
-    revert H.
-    revert t.
-    induction t'; intros.
-    - exfalso. inversion H.
-    - destruct t'.
-      + assert (t = 0) by lia.
-        subst.
-        destruct (f s) eqn:Hl.
-        * left.
-          apply runtime_zero_halted.
-          unfold halted.
-          intros.
-          specialize Hf with s s'.
-          intro.
-          rewrite Hl in Hf.
-          destruct Hf.
-          apply in_nil in H1; auto.
-        * right.
-          intro.
-          unfold halts_within in H0.
-          destruct H0 as [f'].
-          destruct H0.
-          unfold runtime_f in H0.
-          specialize Hf with s s0.
-          destruct Hf.
-          rewrite Hl in H3.
-          remember (H3 (in_eq s0 l)).
-          remember (H0 s s0 (stepsRefl s) s1).
-          lia.
-      + assert (forall (t: nat),
-          t < S t' -> forall s: state, {~halts_within s t} + {~~halts_within s t}
-        ).
-          intros.
-          specialize IHt' with t0 s0.
-          apply IHt' in H0.
-          destruct H0; intuition.
-        destruct (Nat.eq_dec t (S t')).
-        * subst. clear H.
-          assert (t' < S t') by lia.
-          remember (Exists_dec (fun s' => ~halts_within s' t') (f s) (X t' H)).
-          clear Heqs0 X.
-          destruct s0.
-          -- right. intro.
-             apply Exists_exists in e.
-             destruct e.
-             destruct H1.
-             specialize Hf with s x.
-             destruct Hf.
-             remember (H4 H1).
-             exact (H2 (halts_within_step_monotone s x t' s0 H0)).
-          -- left.
-             apply <- Forall_Exists_neg in n.
-             simpl in n.
-             remember (@Forall_forall state (fun x : state => ~ ~ halts_within x t') (f s)).
-             destruct i.
-             remember (n0 n) as H1.
-             clear HeqH1 Heqi f0 n0 n.
-             assert (forall s': state, step_rel s s' -> halts_within s' t').
-             ++ intros.
-                specialize Hf with s s'.
-                specialize IHt' with t' s'.
-                specialize H1 with s'.
-                apply IHt' in H.
-                apply Hf in H0.
-                apply H1 in H0.
-                destruct H; intuition.
-             ++ admit.
-        * assert (t < S t') by lia.
-          exact (IHt' t H0 s).
-  Admitted.
-
-  Local Lemma runtime_exists':
-    next_steps_exists ->
-    forall (t: nat) (initial: state),
-    halts_within initial t -> exists (t': nat), runtime initial t'.
-  Proof.
-    intros.
-    induction t.
-    - exists 0.
-      unfold runtime.
-      intuition.
-      lia.
-    - assert (t < S t) by lia.
-      destruct (halts_within_comp X initial t (S t) H0).
-      + exact (IHt h).
-      + exists (S t).
-        unfold runtime.
-        intuition.
-        assert (t' <= t) by lia.
-        exact (n (halts_within_monotone' initial t' t H3 H2)).
-  Qed.
-
-  Definition decides (l: language): Prop :=
-    forall (w: bitstr), halts' w /\ (accepts w <-> l w).
+  (* simulate correct *)
 End Computation.
 
-
 Section Simulation.
-  Definition dm_steps {state: Type} (dm: @decision_model state) := steps (dm_step dm).
-  Definition dm_halts {state: Type} (dm: @decision_model state) :=
-    halts' (dm_step dm) (dm_enc dm).
+  Definition dm_steps
+    {state: Type} (dm: @decision_model state) := steps (dm_next dm).
+  Definition dm_halts
+    {state: Type} (dm: @decision_model state) := halts (dm_next dm).
+  Definition dm_halted
+    {state: Type} (dm: @decision_model state) := halted (dm_next dm).
+  Definition dm_decision
+    {state: Type} (dm: @decision_model state) := decision (dm_next dm).
+  Definition dm_decides
+    {state: Type} (dm: @decision_model state) := decides (dm_next dm) (dm_enc dm).
 
-  Definition decidable {state: Type} (c: @dm_class state) (l: language) :=
-    exists (dm: decision_model), c dm /\
-    let (step_rel, accepting_state, encode_input) := dm in
-    decides step_rel accepting_state encode_input l.
+  Definition homomorphism
+    {state state': Type} (dm: @decision_model state) (dm': @decision_model state')
+    (h: state -> state') :=
+    (forall (w: bitstr), h (dm_enc dm w) = dm_enc dm' w) /\
+    (forall (s s': state), dm_steps dm s s' -> dm_steps dm' (h s) (h s')) /\
+    (forall (s: state), dm_halted dm s -> dm_halted dm' (h s)) /\
+    (forall (s: state) (b: bool), dm_next dm s = inr b -> dm_next dm' (h s) = inr b).
 
-  Definition simulates {state: Type} (c c': @dm_class state) :=
-    forall (l: language), decidable c' l -> decidable c l.
-
-  Definition homomorphism {state state': Type}
-    (dm: @decision_model state) (dm': @decision_model state') (f: state -> state') :=
-    (forall (w: bitstr), f (dm_enc dm w) = dm_enc dm' w) /\
-    (forall (s: state), dm_acc dm s <-> dm_acc dm' (f s)) /\
-    (forall (s s': state), dm_steps dm s s' -> dm_steps dm' (f s) (f s')).
-
-  Definition homomorphic {state state': Type}
-    (dm: @decision_model state) (dm': @decision_model state') :=
-    exists f, homomorphism dm dm' f.
-
-  Lemma homomorphism_halts {state state': Type}
-    (dm: @decision_model state) (dm': @decision_model state'):
-    homomorphic dm dm' -> forall w, dm_halts dm' w -> dm_halts dm w.
+  Local Lemma homomorphism_decision
+    {state state': Type} (dm: @decision_model state) (dm': @decision_model state')
+    (h: state -> state') (s: state) (b: bool):
+    homomorphism dm dm' h -> dm_decision dm s b -> dm_decision dm' (h s) b.
   Proof.
     intros.
-    destruct dm as [step acc enc].
-    destruct dm' as [step' acc' enc'].
-    unfold dm_halts in *.
-    unfold homomorphic in H.
-    destruct H as [f].
-    destruct H.
-    destruct H1.
-    unfold dm_steps in H2.
+    destruct dm as [next enc].
+    destruct dm' as [next' enc'].
+    unfold homomorphism in H.
+    destruct H. destruct H1. destruct H2.
+    unfold dm_decision in *.
+    unfold dm_halted in *.
+    unfold dm_steps in *.
     simpl in *.
-    unfold halts' in *.
-    unfold halts in *.
-    destruct H0 as [rf].
-    unfold runtime_f in *.
+    induction H0.
+    - apply H3 in H0.
+      repeat econstructor. auto.
+    - assert (steps next s s').
+      + repeat econstructor. auto.
+      + apply H1 in H5.
+        rewrite (steps_decision next' (h s) (h s') b H5).
+        auto.
   Qed.
+
+  Lemma homomorphism_decides
+    {state state': Type} (dm: @decision_model state) (dm': @decision_model state')
+    (h: state -> state') (l: language):
+    homomorphism dm dm' h -> dm_decides dm l -> dm_decides dm' l.
+  Proof.
+    intros.
+    destruct dm as [next enc].
+    destruct dm' as [next' enc'].
+    unfold dm_decides in *.
+    remember H as He. clear HeqHe.
+    destruct He as [Henc H']. clear H'.
+    simpl in *.
+    intro.
+    specialize Henc with w.
+    split.
+    - unfold decides in H0.
+      specialize H0 with w.
+      destruct H0.
+      unfold halts in *.
+      destruct H0.
+      + left.
+        remember H as He. clear HeqHe.
+        apply homomorphism_decision with (s := enc w) (b := true) in H; auto.
+        unfold dm_decision in H. simpl in H.
+        rewrite <- Henc.
+        auto.
+      + right.
+        apply homomorphism_decision with (s := enc w) (b := false) in H; auto.
+        unfold dm_decision in H. simpl in H.
+        rewrite <- Henc.
+        auto.
+    - unfold decides in H0.
+      specialize H0 with w.
+      destruct H0.
+      rewrite <- H1. clear H1.
+      split.
+      + intro.
+        destruct H0; auto.
+        apply homomorphism_decision with (s := enc w) (b := false) in H.
+        unfold dm_decision in H; simpl in H; intros.
+        * rewrite Henc in H.
+          exfalso.
+          apply (decision_unique next' (enc' w)).
+          intuition.
+        * unfold dm_decision. simpl. auto.
+      + intro.
+        apply homomorphism_decision with (s := enc w) (b := true) in H;
+        unfold dm_decision in H; simpl in H; intros.
+        * rewrite <- Henc. auto.
+        * unfold dm_decision. simpl.
+          destruct H0 eqn: Ha; auto.
+  Qed.
+
+  Lemma homomorphism_compose
+    {state state' state'': Type}
+    (dm: @decision_model state) (dm': @decision_model state') (dm'': @decision_model state'')
+    (h: state -> state') (h': state' -> state''):
+    homomorphism dm dm' h -> homomorphism dm' dm'' h' ->
+    homomorphism dm dm'' (fun x => h' (h x)).
+  Proof.
+    intros.
+    destruct dm as [next enc].
+    destruct dm' as [next' enc'].
+    destruct dm'' as [next'' enc''].
+    unfold homomorphism in *.
+    destruct H. destruct H1. destruct H2.
+    destruct H0. destruct H4. destruct H5.
+    unfold dm_decision in *.
+    unfold dm_halted in *.
+    unfold dm_steps in *.
+    simpl in *.
+    split; try split; try split; intros.
+    - rewrite <- H0. rewrite <- H. auto.
+    - apply H4. apply H1. auto.
+    - apply H5. apply H2. auto.
+    - apply H6. apply H3. auto.
+  Qed.
+
+  (*
+     Lemma homomorphism identity
+     Definition class_subset
+     Lemma subset_refl
+     Lemma subset_transitive
+     Lemma subset_subset
+   *)
 
 End Simulation.
