Function.v
@@ -1,0 +1,13 @@
+Require Import Arith List Alphabet.
+
+Section Function.
+  Definition bitstr := list bool.
+  Definition language := bitstr -> Prop.
+  Definition function := nat -> nat.
+
+  Axiom lang_extensionality: forall (l l': language),
+    l = l' <-> forall (w: bitstr), l w <-> l' w.
+
+  Axiom func_extensionality: forall (f f': function),
+    f = f' <-> forall (n: nat), f n = f' n.
+End Function.
