Util.v
@@ -1,0 +1,5 @@
+Require Import Arith Language Lia.
+
+
+Definition isomorphism {A B: Type} (f: A -> B) (finv: B -> A) :=
+  (forall x, finv (f x) = x) /\ (forall x, f (finv x) = x).
